:PROPERTIES:
:ID:       b90b6780-d8c2-4c3a-883e-21aea3a06452
:END:
#+title: LaplaceTransformsExam3
#+OPTIONS: toc:nil num:nil
#+LATEX_HEADER: \usepackage[margin=1in]{geometry}
#+LATEX_HEADER: \usepackage{amsmath}
#+LATEX_HEADER: \usepackage{amssymb}
#+LATEX_HEADER: \setlength{\parindent}{0pt}
#+LATEX_HEADER: \setlength{\parskip}{1em}

* Part 1: Practice Problems

** Question 1 (Inverse Laplace - Partial Fractions)
The inverse Laplace transform of the function
\[ F(s) = \frac{5s+4}{(s-1)(s+2)}\]
is the function $f(t)$.
Find the value of $f(0)$.

\vspace{3cm}

** Question 2 (Inverse Laplace - Quadratic Denominators)
The inverse Laplace transform of the function
\[ F(s) = \frac{3s^2}{(s^2+1)(s^2+4)} \]
is the function $f(t)$.
Find the value of $f(\pi/2)$.

\vspace{3cm}

** Question 3 (IVP - Non-Homogeneous)
Let $y(t)$ be the solution to the initial value problem:
\[ y'' - 3y' + 2y = 6e^{3t} \]
with initial conditions $y(0) = 1$ and $y'(0) = 3$.
Find the value of $y(\ln 2)$.

\vspace{3cm}

** Question 4 (IVP - Coefficient Sum)
Let $y(t)$ be the solution to the initial value problem:
\[ y'' - 4y' + 3y = e^{2t} \]
with initial conditions $y(0) = 2$ and $y'(0) = 3$.
The solution can be written in the form $y(t) = Ae^t + Be^{3t} + Ce^{2t}$.
Find the value of the sum of the coefficients: $A + B + C$.

\vspace{3cm}

** Question 5 (Shifted Laplace)
Let $f(t)$ be the inverse Laplace transform of:
\[ F(s) = \frac{5e^{-2s}}{(s-4)^2} \]
Find the value of $\frac{f(3)}{e^4}$.

#+LATEX: \newpage

* Part 2: Solutions & Answer Key

** Solution to Question 1
We must find the partial fraction decomposition to determine $f(t)$, then evaluate at $t=0$.
\[ \frac{5s+4}{(s-1)(s+2)} = \frac{A}{s-1} + \frac{B}{s+2} \]
Find $A$ (cover-up method at $s=1$):
\[ A = \frac{5(1)+4}{1+2} = \frac{9}{3} = 3 \]
Find $B$ (cover-up method at $s=-2$):
\[ B = \frac{5(-2)+4}{-2-1} = \frac{-6}{-3} = 2 \]
So, $f(t) = 3e^t + 2e^{-2t}$.
Evaluate at $t=0$:
\[ f(0) = 3e^0 + 2e^0 = 3 + 2 = 5 \]
*Answer: 5*

** Solution to Question 2
We assume the form:
\[ \frac{3s^2}{(s^2+1)(s^2+4)} = \frac{A}{s^2+1} + \frac{B}{s^2+4} \]
Multiply by common denominator and substitute $x = s^2$:
\[ 3x = A(x+4) + B(x+1) \]
At $x = -1$: $-3 = A(3) \implies A = -1$.
At $x = -4$: $-12 = B(-3) \implies B = 4$.
\[ F(s) = \frac{-1}{s^2+1} + \frac{4}{s^2+4} \]
Inverse Laplace (remember $\mathcal{L}^{-1}[\frac{\omega}{s^2+\omega^2}] = \sin(\omega t)$):
\[ f(t) = -\sin(t) + \frac{4}{2}\sin(2t) = -\sin(t) + 2\sin(2t) \]
Evaluate at $t = \pi/2$:
\[ f(\pi/2) = -\sin(\pi/2) + 2\sin(\pi) \]
\[ f(\pi/2) = -1 + 2(0) = -1 \]
*Answer: -1*

** Solution to Question 3
1. **Homogeneous:** $r^2 - 3r + 2 = (r-1)(r-2) = 0 \implies y_h = c_1 e^t + c_2 e^{2t}$.
2. **Particular:** Guess $y_p = Ce^{3t}$.
   \[ (9C - 3(3C) + 2C)e^{3t} = 6e^{3t} \implies 2C = 6 \implies C = 3 \]
   General Solution: $y = c_1 e^t + c_2 e^{2t} + 3e^{3t}$.
   Derivative: $y' = c_1 e^t + 2c_2 e^{2t} + 9e^{3t}$.
3. **Initial Conditions:**
   $y(0) = c_1 + c_2 + 3 = 1 \implies c_1 + c_2 = -2$
   $y'(0) = c_1 + 2c_2 + 9 = 3 \implies c_1 + 2c_2 = -6$
   Subtract equations: $c_2 = -4$.
   Solve for $c_1$: $c_1 - 4 = -2 \implies c_1 = 2$.
   Full Solution: $y(t) = 2e^t - 4e^{2t} + 3e^{3t}$.
4. **Evaluate:**
   $y(\ln 2) = 2e^{\ln 2} - 4e^{2\ln 2} + 3e^{3\ln 2}$
   Using $e^{k \ln x} = x^k$:
   $y(\ln 2) = 2(2) - 4(4) + 3(8)$
   $y(\ln 2) = 4 - 16 + 24 = 12$.
*Answer: 12*

** Solution to Question 4
1. **Homogeneous:** $r^2 - 4r + 3 = (r-1)(r-3) \implies y_h = Ae^t + Be^{3t}$.
2. **Particular:** Guess $y_p = Ce^{2t}$.
   \[ (4C - 8C + 3C)e^{2t} = e^{2t} \implies -C = 1 \implies C = -1 \]
   $y = Ae^t + Be^{3t} - e^{2t}$.
   $y' = Ae^t + 3Be^{3t} - 2e^{2t}$.
3. **Initial Conditions:**
   $y(0) = A + B - 1 = 2 \implies A + B = 3$.
   $y'(0) = A + 3B - 2 = 3 \implies A + 3B = 5$.
   Subtract: $2B = 2 \implies B = 1$.
   Solve for $A$: $A + 1 = 3 \implies A = 2$.
   Coefficients are $A=2, B=1, C=-1$.
4. **Sum:**
   $A + B + C = 2 + 1 + (-1) = 2$.
*Answer: 2*

** Solution to Question 5
Base function inverse:
$\mathcal{L}^{-1}\left\{ \frac{5}{(s-4)^2} \right\} = 5te^{4t}$.
Apply time shift $t \to (t-2)$ due to $e^{-2s}$:
$f(t) = 5(t-2)e^{4(t-2)} u(t-2)$.
Evaluate at $t=3$ (note: $u(3-2) = u(1) = 1$):
$f(3) = 5(3-2)e^{4(3-2)} = 5(1)e^4 = 5e^4$.
Compute ratio:
$\frac{5e^4}{e^4} = 5$.
*Answer: 5*
